LinearScan/Basics.hs
@@ -1,6 +1,0 @@
-module LinearScan.Basics where
-
-import qualified Prelude
-import qualified Data.List
-import qualified LinearScan.Utils
-
