LinearScan/List0.hs
@@ -11,18 +11,3 @@ destruct_list l =
   Datatypes.list_rect Prelude.Nothing (\a tail iHtail -> Prelude.Just ((,) a
     tail)) l
 
-fold_left :: (a1 -> a2 -> a1) -> ([] a2) -> a1 -> a1
-fold_left f l a0 =
-  case l of {
-   [] -> a0;
-   (:) b t -> fold_left f t (f a0 b)}
-
-filter :: (a1 -> Prelude.Bool) -> ([] a1) -> [] a1
-filter f l =
-  case l of {
-   [] -> [];
-   (:) x l0 ->
-    case f x of {
-     Prelude.True -> (:) x (filter f l0);
-     Prelude.False -> filter f l0}}
-
