LinearScan/NonEmpty0.hs
@@ -3,8 +3,6 @@ module LinearScan.NonEmpty0 where
 import qualified Prelude
 import qualified Data.List
 import qualified LinearScan.Utils
-import qualified LinearScan.List0 as List0
-
 
 data NonEmpty a =
    NE_Sing a
@@ -42,7 +40,7 @@ coq_NE_last ne =
 
 coq_NE_fold_left :: (a1 -> a2 -> a1) -> (NonEmpty a2) -> a1 -> a1
 coq_NE_fold_left f ne z =
-  List0.fold_left f (coq_NE_to_list ne) z
+  Data.List.foldl' f z (coq_NE_to_list ne)
 
 coq_NE_append :: (NonEmpty a1) -> (NonEmpty a1) -> NonEmpty a1
 coq_NE_append l1 l2 =
