LinearScan/Specif.hs
@@ -12,8 +12,3 @@ type Coq_sig2 a =
   a
   -- singleton inductive, whose constructor was exist2
   
-projT1 :: ((,) a1 a2) -> a1
-projT1 x =
-  case x of {
-   (,) a p -> a}
-
