Vector.v
@@ -1,18 +1,29 @@
 Require Import Coq.Vectors.Vector.
 
-Require Export Ssreflect.ssreflect.
-(* Require Export Ssreflect.ssrfun. *)
-Require Export Ssreflect.ssrbool.
-Require Export Ssreflect.eqtype.
-Require Export Ssreflect.seq.
-Require Export Ssreflect.ssrnat.
-Require Export Ssreflect.fintype.
+Require Import Ssreflect.ssreflect.
+Require Import Ssreflect.ssrfun.
+Require Import Ssreflect.ssrbool.
+Require Import Ssreflect.eqtype.
+Require Import Ssreflect.seq.
+Require Import Ssreflect.ssrnat.
+Require Import Ssreflect.fintype.
 
 Module V := Coq.Vectors.Vector.
-Definition Vec := V.t.
+Notation Vec := V.t.
 
-Definition fin := ordinal.
-Definition vfin := Coq.Vectors.Fin.t.
+(* Extract Inductive Vec => "[]" ["[]" "(\x _ xs -> (x:xs))"]. *)
+
+(* Extract Inlined Constant V.hd      => "(const Prelude.head)". *)
+(* Extract Inlined Constant V.last    => "(const Prelude.last)". *)
+(* Extract Inlined Constant V.tl      => "(const Prelude.tail)". *)
+(* Extract Inlined Constant V.shiftin => "(const Data.List.(:))". *)
+(* Extract Inlined Constant V.const   => "(const Prelude.repeat)". *)
+(* Extract Inlined Constant V.append  => "(\_ _ -> Prelude.(++))". *)
+(* Extract Inlined Constant V.map     => "(const Prelude.map)". *)
+(* Extract Inlined Constant V.nth     => "(const Prelude.nth)". *)
+
+Notation fin := ordinal.
+Notation vfin := Coq.Vectors.Fin.t.
 
 Definition fin_contra : forall {x}, fin 0 -> x.
 Proof.
@@ -27,6 +38,8 @@ Proof.
   by apply/(@Coq.Vectors.Fin.of_nat_lt m)/ltP.
 Defined.
 
+Coercion to_vfin : fin >-> vfin.
+
 Definition fold_left_with_index {A B : Type} {n} (f : fin n -> B -> A -> B) :
   forall (b : B) (v : Vec A n), B.
   intros b v.
@@ -35,3 +48,7 @@ Definition fold_left_with_index {A B : Type} {n} (f : fin n -> B -> A -> B) :
   apply IHv.
   intros. apply X0.
 Defined.
+
+Definition replace {A : Type} {n} v i := @V.replace A _ v (@to_vfin n i).
+
+Definition vnth {A : Type} {n} v i := @V.nth A _ v (@to_vfin n i).
